\documentclass[12pt]{amsart}
\usepackage{amsmath}
\usepackage{amsthm}
\usepackage{amsfonts}
\usepackage{amssymb}
\usepackage{ebproof}
\usepackage[margin=1in]{geometry}
\usepackage{hyperref}
\hypersetup{
    colorlinks=true,
    linkcolor=blue
}

\theoremstyle{definition}
\newtheorem{theorem}{Theorem}[section]
\newtheorem{lemma}[theorem]{Lemma}
\newtheorem{definition}[theorem]{Definition}
\newtheorem{corollary}[theorem]{Corollary}
\newtheorem{proposition}[theorem]{Proposition}
\newtheorem{conjecture}[theorem]{Conjecture}
\newtheorem{remark}[theorem]{Remark}
\newtheorem{example}[theorem]{Example}
\newtheorem{problem}[theorem]{Problem}
\newtheorem{notation}[theorem]{Notation}
\newtheorem{question}[theorem]{Question}
\newtheorem{caution}[theorem]{Caution}

\begin{document}

\title{Homework 2}

\maketitle

\begin{enumerate}
	\item Give natural deduction proofs of the following statements. 

	\begin{enumerate}

	\item $\neg(A \lor B) \to (A \to \neg B)$ 
	\item $\neg A \land \neg B \to \neg (A \lor B)$
	\item $A \leftrightarrow B \vdash \neg A \leftrightarrow \neg B$
	\item $(A \to B) \to (\neg B \to \neg A)$
	\item $((A \to B) \to A) \to A$
	
	\end{enumerate}

	\item Show that $A \to B$, $\neg A \lor B$, and $\neg (A \land \neg B)$ are logically 
		equivalent by writing out truth tables and showing they are the same.

	\item Write out the truth table for $(A \to B) \lor (B \lor C \to A)$. 

\end{enumerate}

\end{document}
